StrataTest/Backends/CBMC/run_tests.sh
@@ -5,7 +5,7 @@ echo "First: tests for the C-like AST interface."
 
 pushd ../../../
 
-echo "Boogie -> CBMC: illustrates verification fail."
+echo "Strata Core -> CBMC: illustrates verification fail."
 echo "----------------------------------------------------------------------"
 Strata/Backends/CBMC/run_strata_cbmc.sh Strata/Backends/CBMC/tests/simpleTest.core.st
 
